$\sin'{x}=\cos{x}$
$\cos'{x}=-\sin{x}$
$\sec'{x}=\sec{x}\times \tan{x}$
$\csc'{x}=-\csc{x}\times \cot{x}$
$\tan'{x}=\sec^2{x}$
$\cot'{x}=-\csc^2{x}$

$(\sin^{-1}{x})'=\frac{1}{\sqrt{1-x^{2}}}$
$(\cos^{-1}{x})'=-\frac{1}{\sqrt{1-x^{2}}}$
$(\sec^{-1}{x})'=\frac{1}{x\sqrt{x^{2}-1}}$
$(\csc^{-1}{x})'=-\frac{1}{x\sqrt{x^{2}-1}}$
$(\tan^{-1}{x})'=\frac{1}{1+x^{2}}$
$(\cot^{-1}{x})'=-\frac{1}{1+x^{2}}$

$(e^x)' = e^x$
$(a^{x})'=a^{x}\times \ln{a}$
$(\ln{x})'=\frac{1}{x}$
$(\log_{a}{x})'=\frac{1}{x\ln{a}}$

**Implicit differentiation:**
$$f(x,y)=g(x,y)\enspace\to\enspace f'(x,y)=g'(x,y)\enspace\to\enspace f'=h(x,y)$$
$(f^{-1})'=\frac{1}{f'\circ f^{-1}}$&ensp;&ensp;&ensp;&ensp;&ensp;($f^{-1}$ here means the inverse function of $f$)

**Product rule**:
$$(f\times g)'=f'\times g+f\times g'$$
**Quotient rule**:
$$(\frac{f}{g})'=\frac{f'\times g-f\times g'}{g^2}$$
**Power rule**:
$$(x^{n})'=nx^{n-1}$$
**Chain rule**:
$$(f\circ g)'=f'\circ g\times g'$$
also
$$(f\circ (g\circ h))'=f'\circ (g\circ h)\times (g'\circ h\times h')$$